src/BBUdiv.v
@@ -8,610 +8,7 @@ Set Implicit Arguments.
 Unset Strict Implicit.
 Import Prenex Implicits.
 
-(* Lemmas *)
-
-(* Lemma dropmsb_zeros : forall n, dropmsb (zeros n) = zeros n.-1. *)
-(* Proof. *)
-(*   move => n. case n. done. *)
-(*   move => n0. have->:(zeros n0.+1.-1=zeros n0) by rewrite-addn1-subn1 addnK. *)
-(*   by rewrite-zeros_rcons/dropmsb/=belastd_rcons.  *)
-(* Qed. *)
-
-
-(* Lemma to_nat_joinlsb a n : to_nat (joinlsb a n) = (to_nat n).*2 + a. *)
-(* Proof. by rewrite addnC. Qed. *)
-
-(* Lemma to_nat_droplsb n: to_nat (droplsb n) = (to_nat n)./2. *)
-(* Proof. elim n=>[|nhd ntl IH]/=. done.  *)
-(*        rewrite -div.divn2 div.divnDr. case nhd ; (rewrite/= div.divn_small; last done). *)
-(*        rewrite add0n; by rewrite -!muln2 div.mulnK.  *)
-(*        rewrite add0n; by rewrite -!muln2 div.mulnK. *)
-(*        rewrite div.dvdn2 odd_double; done. *)
-(* Qed.        *)
-
-
-
-(* Lemma to_nat_joinmsb a n : to_nat (joinmsb n a) = a * 2^(size n) + to_nat n. *)
-(* Proof. *)
-(*   move : a. elim n=>[|nhd ntl IH]a/=. by rewrite -muln2 mul0n !addn0 expn0 muln1.  *)
-(*   rewrite (IH a) -!muln2 mulnDl expnS; ring.  *)
-(* Qed. *)
-
-(* Lemma to_nat_dropmsb n : to_nat (dropmsb (n)) = div.modn (to_nat n) (2^(size n).-1). *)
-(* Proof. *)
-(*   rewrite-(revK n). case (rev n); first by rewrite/= div.modn1. *)
-(*   intros. rewrite/dropmsb/splitmsb/=rev_cons belastd_rcons size_rcons. *)
-(*   have->:((size (rev l)).+1.-1=size (rev l)) by rewrite-addn1-subn1 addnK. *)
-(*   case b; rewrite to_nat_rcons. *)
-(*   - by rewrite mul1n-div.modnDmr div.modnn addn0 (div.modn_small (to_nat_bounded (rev l))). *)
-(*   - by rewrite mul0n addn0 (div.modn_small (to_nat_bounded (rev l))). *)
-(* Qed. *)
-
-
-(* Lemma not_zero_to_nat (q : bits) : (q == zeros (size q))=false -> (to_nat q == 0)=false.   *)
-(* Proof. *)
-(*   intro. apply negbT in H; rewrite -ltB0n ltB_to_nat/= in H. *)
-(*   apply/eqP. rewrite Nat.neq_0_lt_0. apply (Nats.ltn_lt H). *)
-(* Qed. *)
-(* Print div.divn_mulAC. *)
-
-(* Lemma full_mul0n: forall m n, full_mul (zeros m) n = zeros (m + (size n)). *)
-(* Proof. *)
-(*   elim => [|ms IH]n /=. by rewrite from_natn0. *)
-(*   by rewrite (IH n)/joinlsb.  *)
-(* Qed. *)
-  
-(* Lemma full_muln0: forall n m, full_mul n (zeros m) = zeros ((size n) + m). *)
-(* Proof. *)
-(*   elim=>[| nhd ntl IH] m/=. by rewrite from_natn0 size_zeros. *)
-(*   case nhd; rewrite (IH m); first by rewrite zext_zero addB0 unzip1_zip; [ done | by rewrite size_zeros].  *)
-(*   done.   *)
-(* Qed. *)
-  
-(* Lemma mul0B n m: mulB (zeros m) n = zeros m. *)
-(* Proof. *)
-(*   rewrite/mulB full_mul0n/low!size_zeros subnDA subnn sub0n cats0-zeros_cats take_size_cat; [ done | by rewrite size_zeros]. Qed. *)
-
-(* Lemma mulB_nil_l n : mulB [::] n = [::]. *)
-(* Proof. by rewrite/mulB/low/= take0. Qed. *)
-
-(* Lemma full_mul_nil_r n : full_mul n [::]= zeros (size n). *)
-(* Proof. *)
-(*   elim n. done. intros. rewrite/=. case a. rewrite H zext_nil addB0 unzip1_zip; last by rewrite size_joinlsb. done. *)
-(*   by rewrite H. *)
-(* Qed. *)
-
-(* Lemma mulB_nil_r n : mulB n [::] = zeros (size n). *)
-(* Proof.  rewrite/mulB full_mul_nil_r/low size_zeros subnn cats0 take_oversize; last by rewrite size_zeros. done. Qed. *)
-
-(* Lemma zip_nil_r S T (p:seq S) : @zip S T p [::] = [::]. *)
-(* Proof. *)
-(*   case p; done. Qed. *)
-
-(* Lemma full_adder_zip_0_l : forall p n, (full_adder_zip false (zip (zeros n) p)).2 = unzip2 (zip (zeros n) p). *)
-(* Proof. *)
-(*   intros. generalize dependent p. elim n => [|ns IH] p/=. *)
-(*   by rewrite zip_nil.  *)
-(*   elim p => [|phd ptl IH1]/=. done. *)
-(*   case phd; *)
-(*   case Hfadd : (full_adder_zip false (zip (zeros ns) ptl))=>[c tl]/=; *)
-(*   by rewrite -(IH ptl) Hfadd. *)
-(* Qed. *)
-  
-(* Lemma add0B : forall p n, addB (zeros n) p = unzip2 (zip (zeros n) p). *)
-(* Proof. *)
-(*   rewrite /addB/adcB/full_adder.  exact : full_adder_zip_0_l. *)
-(* Qed. *)
-
-(* Lemma to_nat_from_nat_bounded : forall n m, m < 2^n -> to_nat (from_nat n m) = m. *)
-(* Proof. *)
-(*   elim => [|ns IH] m /=. symmetry; rewrite-Nat.lt_1_r; rewrite expn0 in H; by apply Nats.ltn_lt. move => Hlt. *)
-(*   rewrite(IH m./2); last (rewrite expnS Nats.muln_mul in Hlt; rewrite -div.divn2 Nats.divn_div; apply (Nats.lt_ltn (Nat.div_lt_upper_bound m 2 (2^ns)(Nat.neq_succ_0 1) (ltP Hlt)))). *)
-(*   case Hodd: (odd m). *)
-(*   - by rewrite -Hodd odd_double_half.  *)
-(*   - rewrite add0n-div.divn2-muln2 div.divnK; first done. move : (div.dvdn2 m); by rewrite Hodd. *)
-(* Qed. *)
-
-(* Lemma from_nat_bounded_eq m1 m2 n : m1 < 2^n -> m2 < 2^n -> *)
-(*   (m1==m2) = (from_nat n m1 == from_nat n m2). *)
-(* Proof. *)
-(*   move => Hlt1 Hlt2. case E: (m1 == m2); case E': (from_nat n m1 == from_nat n m2) => //. *)
-(*   by rewrite (eqP E) eq_refl in E'. *)
-(*   rewrite -(to_nat_from_nat_bounded Hlt1) -(to_nat_from_nat_bounded Hlt2) in E. *)
-(*   by rewrite (eqP E') eq_refl in E. *)
-(* Qed. *)
-
-(* Lemma from_nat_dhalf n m : joinlsb (odd m) (from_nat n m./2) = from_nat n.+1 m. *)
-(* Proof. done. Qed. *)
-
-(* Lemma from_nat_wrap n : forall m, from_nat n m = from_nat n (m + 2^n). *)
-(* Proof. induction n => //. *)
-(* rewrite expnS. *)
-(* move => m. *)
-(* case ODD: (odd m); rewrite /from_nat-/from_nat /=ODD odd_add odd_mul/=ODD/= halfD ODD/=. *)
-(* specialize (IHn m./2). by rewrite odd_mul/= add0n mul2n doubleK IHn. *)
-(* specialize (IHn m./2). by rewrite add0n mul2n doubleK IHn. *)
-(* Qed. *)
-
-(* Lemma from_nat_wrapMany n c : forall m, from_nat n m = from_nat n (m + c * 2^n). *)
-(* Proof. induction c => m. by rewrite mul0n addn0. *)
-(* rewrite mulSn (addnC (2^n)) addnA from_nat_wrap. rewrite IHc. *)
-(* by rewrite -addnA (addnC (2^n)) addnA. *)
-(* Qed. *)
-
-(* Lemma to_nat_mod p: to_nat p = div.modn (to_nat p) (2^(size p)). *)
-(* Proof. rewrite div.modn_small => //. apply to_nat_bounded. Qed. *)
-
-(* Lemma to_nat_from_nat n m : to_nat (from_nat n m) = div.modn m (2^n). *)
-(* Proof. have H:= div.divn_eq m (2^n). rewrite {1}H. *)
-(* have HH:= from_nat_wrapMany n (div.divn m (2^n)) (div.modn m (2^n)). rewrite addnC in HH. rewrite -HH. *)
-(* rewrite to_nat_from_nat_bounded. done. apply div.ltn_pmod. apply expn_gt0. Qed. *)
-
-(* Lemma adcB_nat p1 p2 c : (adcB c p1 p2).2 = from_nat (size (adcB c p1 p2).2) (c + to_nat p1 + to_nat p2). *)
-(* Proof. *)
-(*   move : p2 c. elim p1 => [|phd1 ptl1 IH1] p2 c/=. *)
-(*   - by rewrite size_adcB/=min0n/=/adcB/full_adder zip_nil. *)
-(*   - move : c. elim p2 => [|phd2 ptl2 IH2] c/=; first done. *)
-(*     move :(IH1 ptl2 c). rewrite/adcB/full_adder/=/bool_adder. *)
-(*     case Hc : c; case Hphd1 : phd1; case Hphd2: phd2; move => Hfazt; *)
-(*     case Hfadderzt : (full_adder_zip true (zip ptl1 ptl2)) =>[c0 tl0]; case Hfadderzf : (full_adder_zip false (zip ptl1 ptl2)) =>[c1 tl1]; try (rewrite Hfadderzt/= in Hfazt; rewrite Hfazt/=). *)
-(*     + rewrite!odd_add!odd_double/= size_from_nat-div.divn2 div.divnDl; last by rewrite div.dvdn2 odd_double. rewrite -2!muln2 (div.mulnK _ (Nats.lt_ltn (Nat.lt_0_succ 1))) (div.divnDr); last by rewrite div.dvdn_mull. rewrite div.divn_small; last done; rewrite add0n div.mulnK; last done. *)
-(*       by rewrite add1n addSn. *)
-(*     + rewrite add0n odd_add!odd_double/=size_from_nat-div.divn2 div.divnDr; last by rewrite div.dvdn2 odd_double. by rewrite-2!muln2!(div.mulnK _ (Nats.lt_ltn (Nat.lt_0_succ 1))) add1n addSn.  *)
-(*     + rewrite add0n uphalf_half!odd_add!odd_double/=size_from_nat-div.divn2 div.divnDl; last by rewrite div.dvdn2 odd_double. rewrite div.divnDr; last by rewrite div.dvdn2 odd_double. rewrite-!muln2!(div.mulnK _ (Nats.lt_ltn (Nat.lt_0_succ 1)))div.divn_small; last done. by rewrite add0n addnA.  *)
-(*     + rewrite-!muln2!add0n-/joinlsb size_joinlsb addn1-from_nat_dhalf-addnA-mulnDl-div.divn2 div.divnDr; last by rewrite div.dvdn2 muln2 odd_double. rewrite div.divn_small; last done. rewrite (div.mulnK _ (Nats.lt_ltn (Nat.lt_0_succ 1))) add0n odd_add muln2 odd_double/=. *)
-(*       move: (IH1 ptl2 false); rewrite/adcB/full_adder Hfadderzf/=add0n. move=>Hfazf; by rewrite Hfazf/=size_from_nat. *)
-(*     + rewrite!add0n-/joinlsb size_joinlsb addn1-from_nat_dhalf!odd_add!odd_double-div.divn2 addnACA div.divnDl; last by rewrite div.dvdn2. rewrite div.divnn/=div.divnDr; last by rewrite div.dvdn2 odd_double. *)
-(*       rewrite-2!muln2!div.mulnK; try done. move : (IH1 ptl2 true); rewrite/adcB/full_adder Hfadderzt/=; move => Hfazf; by rewrite Hfazf size_from_nat addnA. *)
-(*     + rewrite!add0n-/joinlsb size_joinlsb addn1-from_nat_dhalf!odd_add!odd_double-div.divn2!div.divnDr; try by rewrite div.dvdn2 odd_double. rewrite-!muln2!div.mulnK; try done. rewrite div.divn_small/=; try done. *)
-(*       move: (IH1 ptl2 false); rewrite/adcB/full_adder size_full_adder_zip add0n Hfadderzf/=; move => Hfazf; by rewrite Hfazf size_zip size_from_nat. *)
-(*     + rewrite!add0n-/joinlsb size_joinlsb addn1-from_nat_dhalf!odd_add!odd_double-div.divn2 div.divnDl; last by rewrite div.dvdn2 odd_double. rewrite div.divnDr; last by rewrite div.dvdn2 odd_double. rewrite-!muln2!div.mulnK; try done. rewrite div.divn_small/=; try done. move : (IH1 ptl2 false); rewrite/adcB/full_adder Hfadderzf!add0n/=; move => Hfazf; by rewrite Hfazf size_from_nat. *)
-(*     + rewrite!add0n-/joinlsb size_joinlsb addn1-from_nat_dhalf odd_add!odd_double-div.divn2 div.divnDr; last by rewrite div.dvdn2 odd_double. rewrite-!muln2!div.mulnK; try done. move : (IH1 ptl2 false); rewrite/adcB/full_adder Hfadderzf add0n/=; move => Hfazf; by rewrite Hfazf size_from_nat. *)
-(* Qed. *)
-
-(* Corollary to_nat_adcB b p1 p2 : to_nat (adcB b p1 p2).2 = to_nat (from_nat (size (adcB b p1 p2).2) (b + to_nat p1 + to_nat p2)). *)
-(* Proof. *)
-(* rewrite adcB_nat. rewrite size_adcB!to_nat_from_nat size_from_nat=> //.  *)
-(* Qed. *)
-
-(* Lemma to_nat_addB p1 p2 : to_nat (addB p1 p2) = to_nat (from_nat (size (addB p1 p2)) (to_nat p1 + to_nat p2)).  *)
-(* Proof. *)
-(*   rewrite/addB. rewrite to_nat_adcB => //.  *)
-(* Qed.   *)
-
-(* Lemma to_nat_full_mul p1 p2 : to_nat (full_mul p1 p2) = to_nat (from_nat (size (full_mul p1 p2)) (to_nat p1 * to_nat p2)). *)
-(* Proof. *)
-(*   move : p2. elim p1 => [|phd1 ptl1 IH] p2 /=; first by rewrite!from_natn0 size_zeros!add0n.  *)
-(*   move : (to_nat_bounded ptl1) => Hbd1; move : (to_nat_bounded p2) => Hbd2. *)
-(*   move : (Nat.mul_lt_mono _ _ _ _ (ltP Hbd1) (ltP Hbd2)); rewrite-!Nats.muln_mul-expnD; move => Hbd. *)
-(*   SearchAbout lt. move : (mult_S_lt_compat_l 1 _ _  Hbd). rewrite -!Nats.muln_mul mulnC -expnS => Hbdmul. *)
-(*   case phd1. *)
-(*   - rewrite/=to_nat_addB size_addB size_joinlsb to_nat_joinlsb (IH p2) size_full_mul size_zext to_nat_zext addn1-addSn addnC minnn addn0 !to_nat_from_nat-!muln2 div.muln_modl; last done. rewrite addnS expnS. *)
-(*     have-> :(2 * 2 ^ (size p2 + size ptl1) = (2 ^ (size ptl1 + size p2) * 2)) by rewrite mulnC addnC. rewrite div.modnDml. *)
-(*     have->:(((1 + to_nat ptl1 * 2) * to_nat p2) = to_nat ptl1 * to_nat p2 * 2 + to_nat p2) by rewrite mulnDl mul1n; ring. done. *)
-(*   - rewrite size_joinlsb to_nat_joinlsb (IH p2) size_full_mul addn0 add0n-!muln2!to_nat_from_nat_bounded; first ring. rewrite addn1 mulnAC. apply/ltP; exact. apply/ltP; exact.  *)
-(* Qed. *)
-
-(* Lemma to_nat_take : forall n p, to_nat ((take n) p) = if n < size p then to_nat (from_nat n (to_nat p)) else to_nat p. *)
-(*   elim => [| ns IH] p. *)
-(*   rewrite take0/=. *)
-(*   elim p => [| phd ptl IHm]; done. *)
-(*   elim p => [| phd ptl IHm]; first done. *)
-(*   rewrite to_nat_cons/=. *)
-(*   case Hlt : (ns.+1 < (size ptl).+1); rewrite ltnS in Hlt.  *)
-(*   rewrite odd_add odd_double oddb. rewrite (IH ptl) Hlt. *)
-(*   case phd; first by rewrite/=uphalf_double.  *)
-(*   by (rewrite/=3!add0n-3!muln2-div.divn2 div.mulnK; last done). *)
-(*   by rewrite IH Hlt. *)
-(* Qed. *)
-
-(* Lemma to_nat_mulB p1 p2 : to_nat (mulB p1 p2) = to_nat (from_nat (size p1) (to_nat p1 * to_nat p2)). *)
-(* Proof. *)
-(*   rewrite/mulB/low size_full_mul to_nat_cat to_nat_zeros mul0n addn0 to_nat_take size_full_mul. *)
-(*   case Hlt : (size p1 < size p1 + size p2). *)
-(*   by rewrite to_nat_full_mul size_full_mul 3!to_nat_from_nat expnD Nats.modn_muln_modn_l.  *)
-(*   rewrite to_nat_full_mul size_full_mul. *)
-(*   have Hadd0 : size p1 = size p1 +0 by rewrite addn0. rewrite {1}Hadd0 ltn_add2l in Hlt. *)
-(*   move/negP/negP: Hlt. rewrite-eqn0Ngt. move/eqP => Hlt. by rewrite Hlt addn0. *)
-(* Qed. *)
-  
-(* Lemma mulnB_eq0: forall m n : bits, (mulB m n == (zeros (size m))) = (m == zeros (size m)) || (n == zeros (size n)). *)
-(* Proof. *)
-(*   intros. *)
-(*   case Hmz : (m == zeros (size m)). *)
-(*   - by rewrite (eqP Hmz) mul0B size_zeros eq_refl. *)
-(*   - case Hnz : (n == zeros (size n)). *)
-(*     + rewrite (eqP Hnz)/mulB full_mul0/low size_zeros subnDA subnn sub0n cats0-zeros_cats take_size_cat/= ; last by rewrite size_zeros. exact: eq_refl. *)
-(*     + move : Hmz Hnz. move : n. *)
-(*       elim m => [|mhd mtl IH]n/=. by rewrite mulB_nil_l. *)
-(*   rewrite /mulB/=. case Hmhd: mhd. intros. *)
-(*   move : (IH n). rewrite/mulB/low size_addB size_joinlsb size_zext!size_full_mul addnAC addn1 subnDA subnn sub0n cats0. intros. rewrite addnC minnn subnDA subnAC subnn sub0n cats0. rewrite (take_nth false).  *)
-(* Admitted. *)
-
-
-
-(* Lemma subB_is_dropmsb_adcB_invB (p q: bits) : subB p q = dropmsb (adcB true p (invB q)).2. *)
-(* Proof.  *)
-(* Admitted. *)
-
-(* Lemma sub0B : forall m, subB (zeros (size m)) m = negB m. *)
-(* Proof. *)
-(*   elim => [|mhd mtl IH]/=. done. *)
-(*   case mhd. rewrite/subB/sbbB/adcB/full_adder/=. *)
-(*   case Hfaddzf : (full_adder_zip false (zip (zeros (size mtl)) (~~# mtl)%bits))=>[c res]/=. *)
-(*   have -> : res = (full_adder_zip false (zip (zeros (size mtl)) (~~# mtl)%bits)).2 *)
-(*     by rewrite Hfaddzf. *)
-(*   rewrite full_adder_zip_0_l unzip2_zip ; last by rewrite size_zeros -BBNeg.invB_size_ss. *)
-(* Admitted. *)
-  
-(* Lemma subB0: forall m n, subB m (zeros n) = m. *)
-(* Proof. *)
-(* Admitted. *)
-  
-(* Lemma mulB0' : forall m n, mulB m (zeros n) = zeros (size m). *)
-(* Proof. *)
-(*   intros. rewrite/mulB full_muln0/low -zeros_cats take_cat size_zeros/=. *)
-(*   case H : (size m < size m). move : (Nat.lt_irrefl (size m))=>Heq. *)
-(*   exfalso; apply Heq; apply Nats.ltn_lt; rewrite H; done. *)
-(*   by rewrite size_cat size_zeros subnDA subnn take0 sub0n !cats0. *)
-(* Qed. *)
-
-(* Lemma to_nat_shlB1 : forall (p: bits), to_nat (shlB1 p) = div.modn ((to_nat p).*2) (2^size p). *)
-(* Proof. move => p. by rewrite /shlB1 to_nat_dropmsb to_nat_joinlsb size_joinlsb-subn1 addnK addn0-muln2. *)
-(* Qed. *)
-
-(* Lemma to_nat_shlBn: *)
-(*   forall n k, k < n -> to_nat (shlB k (from_nat n 1) ) = 2 ^ k. *)
-(* Proof. *)
-(* Admitted. *)
-
-(* Lemma shlB_dropmsb n (p: bits) : shlB n (dropmsb p) = dropmsb (shlB n p). *)
-(* Proof. *)
-(* Admitted. *)
-
-(* Lemma to_nat_shrB1 : forall bs, to_nat (shrB1 bs) = div.divn (to_nat bs) 2. *)
-(* Proof. *)
-(*   elim => [|bhd btl IH]/=. done. *)
-(*   by rewrite/shrB1 to_nat_droplsb to_nat_joinmsb mul0n add0n/=-muln2-div.divn2. *)
-(* Qed. *)
-  
-(* Lemma to_nat_shrB : forall n bs, to_nat (shrB n bs) = div.divn (to_nat bs) (2^n). *)
-(* Proof. *)
-(*   intros. *)
-(*   elim n => [|ns IH]/=. by rewrite div.divn1. *)
-(*   by rewrite to_nat_shrB1 IH-div.divnMA expnS mulnC.  *)
-(* Qed. *)
-  
-
 (* ===== bit_blast_udiv ===== *)
-
-(*Fixpoint act_size' (b : bits) : nat :=
-  match b with
-  | [::] => 0
-  | bhd :: btl => if bhd then size b else act_size' btl
-  end.
-
-Definition act_size b := act_size' (rev b).
-
-Fixpoint act_sizel' (l : word) :=
-  match l with
-  |[::] => 0
-  | lhd :: ltl => if (lhd==lit_tt) then size l else act_sizel' ltl
-  end.
-
-Definition act_sizel l := act_sizel' (rev l).
-*)
-(*Fixpoint udivB_rec (n m : bits) i : bits * bits :=
-  match i with
-  | 0 => (zeros (size n), shrB (act_size n - (act_size m) + 1) n)
-  | S i' => 
-    let ai := nth false n (act_size n - i' - (act_size m)) in
-    let di := dropmsb (joinlsb ai (udivB_rec n m i').2 ) in
-    let bi := negb (ltn (to_nat di) (to_nat m)) in
-    let ri := if bi then subB di (zext (size di - size m) m) else di in
-    let qi := dropmsb (joinlsb bi (udivB_rec n m i').1) in
-    (qi, ri)
-  end.
-
-Definition udivB (n m : bits) :=
-  if (m == zeros (size m)) then (zeros (size n), zeros (size n))
-  else  udivB_rec n m `(act_size n - (act_size m) + 1).*)
-
-
-(* Fixpoint udivB_rec (n m : bits) (q r : bits): bits * bits := *)
-(*   match n with *)
-(*   | [::] => (q, r) *)
-(*   | nhd :: ntl => let di := dropmsb (joinlsb nhd r) in *)
-(*                   let bi := negb (ltn (to_nat di) (to_nat m)) in *)
-(*                   let ri := if bi then subB di m else di in *)
-(*                   let qi := dropmsb (joinlsb bi q) in *)
-(*                   udivB_rec ntl m qi ri *)
-(*   end. *)
-
-(* Definition udivB (n' m : bits) : bits * bits := *)
-(*   let n := rev n' in *)
-(*   if ((from_nat (size n) (to_nat m)) == zeros (size n)) then (zeros (size n), n') *)
-(*   else udivB_rec n (from_nat (size n) (to_nat m)) (zeros (size n)) (zeros (size n)). *)
-
-(*Definition udivB_extzip (zip : seq (bool * bool)) (q r : bits) : bits * bits :=
-  udivB_rec (rev (unzip1 zip)) (unzip2 zip) q r .
-
-Definition udivB (n m : bits) : bits * bits :=
-  if (m == zeros (size m)) then (zeros (maxn(size n)(size m)), unzip1 (extzip0 n m))
-  else udivB_extzip (extzip0 n m) (zeros (maxn(size n)(size m))) (zeros (maxn(size n)(size m))).*)
-
-(* Eval compute in (to_nat (udivB (from_nat 8 185) (from_nat 4 13)).1). *)
-(* Eval compute in (to_nat (udivB (from_nat 8 185) (from_nat 4 13)).2). *)
-(* Eval compute in (to_nat (udivB (from_nat 8 156) (from_nat 3 2)).1). *)
-(* Eval compute in (to_nat (udivB (from_nat 8 16) (from_nat 3 2)).2). *)
-
-
-(* Lemma size_udivB_rec n m q r : size (udivB_rec n m q r).1 = size q. *)
-(* Proof. *)
-(*   move : m q r.  elim n => [|nhd ntl IH]m q r/=; first done.  *)
-(*   rewrite (IH m (dropmsb (joinlsb (~~ (to_nat (dropmsb (joinlsb nhd r)) < to_nat m)) q)) *)
-(*               (if ~~ (to_nat (dropmsb (joinlsb nhd r)) < to_nat m) *)
-(*                then (dropmsb (joinlsb nhd r) -# m)%bits *)
-(*                else dropmsb (joinlsb nhd r))). *)
-(*     by rewrite size_dropmsb size_joinlsb addnK. *)
-(* Qed.   *)
-
-(* Lemma size_udivB n m : size (udivB n m).1 = (size n). *)
-(* Proof. *)
-(*   rewrite/udivB. case Hm0: ((size (rev n)) -bits of (to_nat m)%bits == zeros (size (rev n))); first by rewrite size_rev size_zeros. *)
-(*   by rewrite size_udivB_rec size_zeros size_rev. *)
-(* Qed. *)
-
-(* Lemma udivB_rec0r : forall m n q r,  (udivB_rec m (zeros n) q r) = (addB (shlB (size m) q) (zext (size q - size m) (ones (size m))), addB (shlB (size m) r) (zext (size r - size m) (rev m))). *)
-(* Proof.  *)
-(*   elim => [|mhd mtl IH] n q r; rewrite/=. rewrite/rev/=!zext_nil!subn0!addB0 unzip1_zip; last by rewrite size_zeros. rewrite unzip1_zip; last by rewrite size_zeros. done. *)
-(*   intros. rewrite to_nat_zeros/=subB0.  *)
-(*   rewrite IH; first rewrite size_dropmsb size_joinlsb addnK.  *)
-(*   rewrite /shlB1. *)
-(*   assert ((dropmsb (joinlsb true q) <<# size mtl +# zext (size q - size mtl) (ones (size mtl)))%bits==(dropmsb (joinlsb false (q <<# size mtl)) +# zext (size q - (size mtl).+1) (b1 :: ones (size mtl)))%bits). *)
-(*   rewrite shlB_dropmsb-to_nat_inj_ss; last by rewrite!size_addB!size_dropmsb!size_zext/=size_ones!size_shlB size_joinlsb addnK -addn1 addnK; repeat rewrite-maxnE maxKn. *)
-(*   rewrite 2!to_nat_addB 2!to_nat_zext/=to_nat_ones 2!to_nat_dropmsb to_nat_joinlsb. rewrite/shlB 2!shlB_mul2exp 2!to_nat_mulB addn0.   *)
-(*   rewrite 2!size_addB 2!size_dropmsb 2!size_joinlsb 2!size_mulB size_joinlsb 2!size_zext-subn1 addnK/= size_ones-!maxnE !maxKn. *)
-(*   rewrite !to_nat_from_nat. *)
-(* Admitted. *)
-  
-  
-(* Lemma udivB0 : forall n m, (udivB m (zeros n)) = (zeros (size m), m). *)
-(* Proof. *)
-(*   intros; rewrite/udivB. by rewrite to_nat_zeros from_natn0 eq_refl size_rev.  *)
-(* Qed. *)
-
-
-(* Lemma udivB_rec0_aux : forall n(m : bits) s, *)
-(*     ~~(m==zeros(size m)) -> udivB_rec (zeros n) m (zeros s) (zeros s)= (zeros s, zeros s). *)
-(* Proof. *)
-(*   elim. intros; first by done. *)
-(*   intros. rewrite-zeros_cons/=to_nat_dropmsb to_nat_joinlsb to_nat_zeros div.mod0n.  *)
-(*   move : (to_nat_zero m). move: H0; rewrite-eqbF_neg; move=>Hnotz; rewrite(eqP Hnotz)eqn0Ngt; move=>Htonat; rewrite Htonat/joinlsb zeros_cons dropmsb_zeros-pred_Sn. rewrite eqbF_neg in Hnotz. *)
-(*   exact :(H m s Hnotz). *)
-(* Qed. *)
-
-
-  
-(* Lemma udivB_rec0 : forall n (m : bits) q r , *)
-(*     ~~(m==zeros(size m)) -> udivB_rec (zeros n.+1) m q (zeros r)= (shlB n.+1 q, (zeros r)). *)
-(* Proof. *)
-(*   intros. rewrite-zeros_cons/=to_nat_dropmsb to_nat_joinlsb to_nat_zeros div.mod0n. *)
-(*   move : (to_nat_zero m). move: H; rewrite-eqbF_neg; move=>Hnotz; rewrite(eqP Hnotz)eqn0Ngt; move=>Htonat; rewrite Htonat/joinlsb zeros_cons dropmsb_zeros-pred_Sn/shlB1. rewrite eqbF_neg in Hnotz. *)
-(*   move: q r. elim n; first done.  intros. rewrite-zeros_cons/=to_nat_dropmsb to_nat_joinlsb to_nat_zeros div.mod0n Htonat/joinlsb zeros_cons dropmsb_zeros-addn1-subn1 addnK. *)
-(*   move :(H (dropmsb (false :: q)) r).  *)
-(*   rewrite/shlB1/joinlsb. have->: ((dropmsb (false :: q) <<# n0)%bits = dropmsb (false :: (q <<# n0)%bits)). *)
-(*   rewrite/shlB/shlB1. elim n0; first done. rewrite/joinlsb/=; intros; by rewrite H0. *)
-(*   done. *)
-(* Qed. *)
-
-(* Lemma rev_copy : forall T n (b: T), rev (copy n b) = copy n b. *)
-(* Proof. *)
-(* Admitted. *)
-  
-(* Lemma udiv0B : forall n (m: bits), ~~(from_nat n (to_nat m) == zeros n)-> udivB (zeros n) m = (zeros n, zeros n). *)
-(* Proof. *)
-(*   move => n m Hm. move : (negbTE Hm) => Hnot0. rewrite/udivB size_rev size_zeros Hnot0.  *)
-(*   move : Hnot0. elim n; first done. *)
-(*   move => ns Hudiv Hnot0.  rewrite rev_copy udivB_rec0; first by rewrite/shlB shlB_mul2exp mul0B. *)
-(*   by rewrite size_from_nat Hnot0. *)
-(* Qed. *)
-  
-(* Lemma size_uremB_rec : forall  n m q r, size m = size r -> size (udivB_rec n m q r).2 = size r. *)
-(* Proof. *)
-(*   elim =>[|nhd ntl IH]m q r Hsz; first done. *)
-(*   rewrite/=(IH m (dropmsb (joinlsb (~~ (to_nat (dropmsb (joinlsb nhd r)) < to_nat m)) q)) *)
-(*        (if ~~ (to_nat (dropmsb (joinlsb nhd r)) < to_nat m) *)
-(*         then (dropmsb (joinlsb nhd r) -# m)%bits *)
-(*         else dropmsb (joinlsb nhd r))); *)
-(*   case H : ((to_nat (dropmsb (joinlsb nhd r)) < to_nat m)); try (by rewrite/=size_dropmsb size_joinlsb addnK|| by rewrite/=size_subB size_dropmsb size_joinlsb addnK Hsz minnn). *)
-(* Qed.     *)
-
-(* Lemma size_uremB : forall n m , size (udivB n m).2 = size n. *)
-(* Proof. *)
-(*   rewrite/udivB. intros. *)
-(*   case Hm0: ((size (rev n)) -bits of (to_nat m)%bits == zeros (size (rev n))); first done.  *)
-(*   rewrite size_rev size_uremB_rec; rewrite size_zeros; first done. by rewrite size_from_nat. *)
-(* Qed.   *)
-
-(* Lemma udivB_mulAC : forall d m n, (udivB d m).2 = zeros (size d) -> udivB m (mulB d n) = udivB (mulB m n) d. *)
-(* Proof. *)
-(*   elim =>[|dhd dtl IH] m n H; rewrite/udivB/=. *)
-(*   - rewrite !size_mulB/mulB/= /low !take0 add0n sub0n zeros0 cats0/=/extzip0!unzip1_extzip!sub0n!cats0.  *)
-(*   - case Hz : (dhd :: dtl == b0 :: zeros (size dtl)). *)
-(*     + rewrite (eqP Hz)zeros_cons size_mulB size_zeros !mul0B/=. *)
-(*       case Hzeros: (b0 :: zeros (size dtl) == b0 :: zeros (size dtl)); rewrite !size_mulB; first done. *)
-(*       rewrite zeros_cons in Hzeros. move : (eq_refl (zeros (size dtl).+1)) => Hzeros'; rewrite Hzeros' in Hzeros; discriminate. *)
-(*     + case Hmul0 : (((dhd :: dtl) *# n)%bits == zeros (size ((dhd :: dtl) *# n)%bits)). *)
-(*       * rewrite size_mulB mulnB_eq0 in Hmul0. move : (orP Hmul0)=>[Hl| Hr]. *)
-(*         rewrite/= in Hl. rewrite Hl in Hz; discriminate. *)
-(*         rewrite (eqP Hr) mulB0' act_size0 sub0n add0n. rewrite/=subn0 !act_size0 !sub0n add0n size_zeros nth0. have ->: (head false (zeros (size m))=false) by (case m=>[|mhd mtl]; by rewrite/=). rewrite/joinlsb/=/shrB1/= to_nat_dropmsb/=to_nat_droplsb/= to_nat_joinmsb mul0n to_nat_zeros addn0 div.mod0n. move : (to_nat_zero (dhd :: dtl))=> Heqz. rewrite Hz/= in Heqz. rewrite (neq0_lt0n Heqz)/= zeros_cons dropmsb_zeros. by rewrite/joinmsb zeros_rcons /droplsb/=zeros_cons dropmsb_zeros-addn1-subn1 addnK. *)
-(*       * rewrite size_mulB mulnB_eq0 Hz/= in Hmul0. *)
-
-(* Admitted. *)
-  
-
-
-(* Lemma ltn_neq0 : forall n m, n < m -> (m != 0). *)
-(* Proof. *)
-(*   elim => [| ns IH] m/=. by rewrite lt0n. *)
-(*   - intro. rewrite-(eqP (Nats.lt_sub1r_add1l ns m)) in H; apply (IH m.-1) in H. *)
-(*     rewrite-lt0n (eqP (Nats.lt_sub1r_add1l 0 m)) in H. move : (ltn_trans (ltn0Sn 0) H). by rewrite lt0n. *)
-(* Qed. *)
-
-(* Lemma lt0B_size : forall b, ([::] <# b)%bits -> 0 < size b. *)
-(* Proof. *)
-(*   elim; first done. intros; by rewrite ltn0Sn. *)
-(* Qed. *)
-
-(* Lemma odd_to_nat_lsb : forall b, odd (to_nat b) =lsb b. *)
-(* Proof. *)
-(*   elim; first by rewrite/lsb/splitlsb/=. *)
-(*   move => a l IH. *)
-(*   rewrite/lsb/=odd_add odd_double-negb_eqb. case Ha : a; done. *)
-(* Qed. *)
-
-(* Lemma neq0_eq0_sizel : forall n (b : bits), b!=zeros (size b) -> from_nat n (to_nat b) == zeros n -> n < size b. *)
-(* Proof. *)
-(*   elim => [|ns IH] b/=; first by (rewrite-ltB0n eq_refl; move=> [Hneq Ht{Ht}]; exact (lt0B_size Hneq)). *)
-(*   move=>[Hneq Heq]. move : (IH (droplsb b)) => Hm. rewrite-(eqP (Nats.lt_sub1r_add1l ns (size b)))-subn1-size_droplsb. apply Hm; last rewrite to_nat_droplsb. *)
-(*   move : Hneq. rewrite-!to_nat_zero to_nat_droplsb-!lt0n half_gt0. move => Hgt0. *)
-(*   case Hoddb: (odd (to_nat b)); first by rewrite Hoddb eqseq_cons andFb in Heq. *)
-(*   rewrite Hoddb/joinlsb eqseq_cons andTb in Heq. rewrite Nats.ssrodd_odd-Nat.even_succ-Nat.negb_odd in Hoddb. move: (negbFE Hoddb)=>Hodd{Hoddb}. rewrite-Nats.ssrodd_odd in Hodd. rewrite-(ltn_add2r 1)2!addn1 in Hgt0. move : (odd_gt2 Hodd Hgt0)=> Hodd2.  move : (ltn_sub2r Hgt0 Hodd2). by rewrite!subn1/=.  *)
-(*   rewrite eqseq_cons in Heq. move/andP : Heq=>[Hb0 Hzeq]. done. *)
-(* Qed. *)
-
-
-(* Lemma to_nat_belast_0 : forall s, to_nat (belast false (zeros s)) = 0. *)
-(* Proof. *)
-(*   elim => [|ns IH]/=; first done. rewrite IH-muln2 mul0n; done. *)
-(* Qed. *)
-
-(* Lemma lt1_eq0 : forall (n:nat), n<1 -> n=0. *)
-(* Proof. intros. induction n; try done. *)
-(* Qed. *)
-
-
-(* Lemma subB_joinmsb_dropmsb: forall b q n, size q = n.+1 -> (dropmsb (joinlsb b q) -# joinlsb b (zeros n))%bits = dropmsb (joinlsb false q). *)
-(* Proof. *)
-(* Admitted. *)
- (* 
-Lemma udivB_rec1 : forall p s q r, p!=[::]->size r = s -> udivB_rec p (from_nat s 1) q r = (q, dropmsb (joinlsb (msb p) r)).
-Proof.
-  elim => [|ph pt IH]/=; first discriminate.
-  move => s q r Hp Hsz.
-  rewrite IH.
-  move : Hsz. Print udivB_rec. case Hs : s=>[|ns]; rewrite/=. rewrite-zeros0 subB0. intros.
-  move : (size0nil Hsz)=> Hrnil. rewrite Hrnil/joinlsb{2}/dropmsb/msb{-1}/dropmsb/=.
-  (*(dropmsb (true :: q), [::]) = (q, [::])*) admit.
-  rewrite from_natn0 to_nat_zeros-muln2 mul0n addn0. 
-  case Hph : ph; rewrite/=; intro.
-  destruct r; rewrite/=; first discriminate.
-  rewrite subB_joinmsb_dropmsb; last done. rewrite/msb/=.
-  
-  
-  (*(dropmsb (joinlsb true q),
-  (dropmsb (joinlsb true (a :: r)) -# joinlsb true (zeros ns))%bits) = 
-  (q, a :: r)*) admit.
-  destruct r; first discriminate.
-  case Hbr1 : (to_nat (dropmsb (joinlsb false (b :: r))) < 1).
-  move/eqP: Hbr1. rewrite-addn1 addnK. move=> Hbr1.
-  rewrite/=.
-  (*(dropmsb (joinlsb false q), dropmsb (joinlsb false (b :: r))) = (q, b :: r)*) admit.
-  rewrite/=. 
-  (*(dropmsb (joinlsb true q),
-  (dropmsb (joinlsb false (b :: r)) -# joinlsb true (zeros ns))%bits) = 
-  (q, b :: r)*)
-  admit.
-  case Hlt : (to_nat (dropmsb (joinlsb ph r)) < to_nat (s) -bits of (1)%bits); rewrite/=.
-  by rewrite size_dropmsb size_joinlsb addnK Hsz.
-  by rewrite QFBV.size_subB size_dropmsb size_joinlsb addnK Hsz size_from_nat minnn.
-*)
-
-  
-(* Lemma udivB1: forall p, udivB p (from_nat (size p) 1) = (p, from_nat (size p) 0). *)
-(* Proof. *)
-(*   elim=>[| ph pt IH]/=; first done.  *)
-(*   rewrite/udivB!from_natn0 to_nat_joinlsb to_nat_zeros-muln2 mul0n add0n. *)
-(*   rewrite-from_natn0 -from_nat_bounded_eq; [|by rewrite/=size_rev Nats.expn2_gt1|by rewrite size_rev Nats.expn2_gt0]. *)
-(*   rewrite/udivB in IH. *)
-(*   rewrite/=!from_natn0 size_rev/=.  *)
-(* Admitted. *)
-  
-(* Lemma shrB_div2exp:  forall i p , (iter i shrB1 p, from_nat (size p) 0) = udivB p (from_nat (size p) (2^ i)%nat). *)
-(* Proof. *)
-(* Admitted. *)
-  
-(* Lemma udivB_def: forall q d r, ltB r d -> (udivB (addB (mulB q d) r) d).2 = r. *)
-(* Proof. *)
-(* Admitted. *)
-  
-(* Lemma udivB_rec_to_nat : forall nhd ntl m q r, to_nat (udivB_rec (nhd::ntl) m q r).1 = addn (div.divn (addn (to_nat (shlB (size ntl).+1 r)) (to_nat (nhd::ntl))) (to_nat m)) (to_nat q). *)
-(* Proof. *)
-(* Admitted. *)
-  
-(* Lemma udivB_to_nat : forall p q,  to_nat (udivB p q).1 = (div.divn (to_nat p) (to_nat (from_nat (size p) (to_nat q)))). *)
-(* Proof. *)
-  
-(*   intros. rewrite/udivB. *)
-(*   case H0 : ((size p) -bits of (to_nat q)%bits == zeros (size p)); *)
-(*     first by rewrite/=(eqP H0) to_nat_zeros div.divn0.  *)
-(*   move : q H0. elim p =>[|phd ptl IH] q H0/=; first done. *)
-(*   have : (to_nat (dropmsb (zeros (size ptl).+1)) = 0) by rewrite to_nat_dropmsb to_nat_zeros div.mod0n. *)
-(*   rewrite/dropmsb/splitmsb/=; move => Hbelast; rewrite Hbelast-muln2 mul0n addn0/=. *)
-(*   case Hphd : phd; case Hoddq : (odd (to_nat q)); rewrite /=eqseq_cons Hoddq in H0; rewrite/=. *)
-(*   - have Hgt0 : (0 < (to_nat (size ptl) -bits of ((to_nat q)./2)%bits)). admit. *)
-(*     move : (muln_gt0 (to_nat (size ptl) -bits of ((to_nat q)./2)%bits) 2)=> Hgt0'; rewrite Hgt0(ltn0Sn 1)andTb muln2-(ltn_add2l 1)addn0 in Hgt0'. *)
-(*     rewrite Hgt0'/=. *)
-
-    
-(*     rewrite Hgt0' udivB_rec_to_nat/shlB shlB_mul2exp/=add0n/mulB/=size_belast size_zeros/low size_addB size_joinlsb.  *)
-
-(* Admitted.   *)
-
-(* Lemma uremB_to_nat : forall p q , to_nat (udivB p q).2 = (div.modn (to_nat p) (to_nat q)). *)
-(* Proof.   *)
-(* Admitted. *)
-
-(*
-Fixpoint bit_blast_udiv_rec_t g ls1 ls2 cs qs rs: generator * cnf * word * word :=
-
-  match ls1 with
-  | [::] => (g, cs, qs, rs)
-  | ls_hd1 :: ls_tl1 =>
-    let di := dropmsl (joinlsl ls_hd1 rs) in
-    let '(g_ge, cs_ge, lrs_ge) := bit_blast_uge g di ls2 in
-    let qi := dropmsl (joinlsl lrs_ge qs) in
-    if (lrs_ge==lit_tt) then
-      let '(g_sub, cs_sub, lrs_sub) := bit_blast_sub g_ge di ls2 in
-      bit_blast_udiv_rec_t g_sub ls_tl1 ls2 (catrev (catrev cs cs_ge) cs_sub) qi lrs_sub
-    else if (lrs_ge == lit_ff) then bit_blast_udiv_rec_t g_ge ls_tl1 ls2 (catrev cs cs_ge) qi di
-         else
-           let '(g_and, cs_and, lrs_and) := bit_blast_and g_ge (copy (size ls2) lrs_ge) ls2 in
-           let '(g_sub2, cs_sub2, lrs_sub2) := bit_blast_sub g_and di lrs_and in
-           bit_blast_udiv_rec_t g_sub2 ls_tl1 ls2 (catrev (catrev (catrev cs cs_ge) cs_and) cs_sub2) qi lrs_sub2
-  end.
-*)
-
-(*
-Fixpoint bit_blast_udiv_rec g ls1 ls2 qs rs :  generator * cnf * word * word :=
-  match ls1 with
-  | [::] => (g, [::], qs, rs)
-  | ls1_hd :: ls1_tl =>
-    let '(g_tl, cs_tl, lrs_tl, lqs_tl) := bit_blast_udiv_rec g ls1_tl ls2 qs rs in
-    let di := dropmsl (joinlsl ls1_hd lrs_tl) in
-    let '(g_hd, cs_hd, lrs_hd) := bit_blast_uge g_tl di ls2 in
-    let qi := dropmsl (joinlsl lrs_hd lqs_tl) in
-    if (lrs_hd == lit_tt) then
-      let '(g_sub, cs_sub, lrs_sub) := bit_blast_sub g_hd di ls2 in
-      (g_sub, (catrev (catrev cs_tl cs_hd) cs_sub), qi, lrs_sub)
-    else if (lrs_hd == lit_ff) then
-           (g_hd, catrev cs_tl cs_hd, qi, di)
-         else let '(g_and, cs_and, lrs_and) := bit_blast_and g_hd (copy (size ls2) lrs_hd) ls2 in
-              let '(g_sub2, cs_sub2, lrs_sub2) := bit_blast_sub g_and di lrs_and in
-              (g_sub2, (catrev (catrev (catrev cs_tl cs_hd) cs_and) cs_sub2), qi, lrs_sub2)
-  end.
-*)
 
 
 Fixpoint bit_blast_udiv_rec g ls1 ls2 qs rs :  generator * cnf * word * word :=
@@ -634,8 +31,6 @@ Fixpoint bit_blast_udiv_rec g ls1 ls2 qs rs :  generator * cnf * word * word :=
               (g_tl, (catrev (catrev (catrev cs_tl cs_sub2) cs_and) cs_uge), lrs_tl, lqs_tl)
   end.             
 
-Compute ( (udivB_rec [:: true; false; true; false] (zeros 4) (zeros 4) (zeros 4))).
-
 Definition bit_blast_udiv g ls1' ls2 :=
   let ls1 := rev ls1' in
   let '(g_eq, cs_eq, lrs_eq) := bit_blast_eq g ls2 (copy (size ls2) lit_ff) in
@@ -651,6 +46,9 @@ Definition bit_blast_udiv g ls1' ls2 :=
          let '(g_and, cs_and, lrs_and) := bit_blast_and g_udivr (copy (size lqs_udivr) (neg_lit lrs_eq)) lqs_udivr  in
          let '(g_ite, cs_ite, lrs_ite) := bit_blast_ite g_and lrs_eq (rev lrs_udivr) lrs_udivr in
          (g_ite, catrev (catrev (catrev cs_ite cs_and) cs_udivr) cs_eq, lrs_and, lrs_ite).
+
+Definition bit_blast_udiv' g ls1 ls2 :=
+  let '(g_udiv, cs_udiv, q_udiv, r_udiv) := bit_blast_udiv g ls1 ls2 in (g_udiv, cs_udiv, q_udiv).
 
 Fixpoint mk_env_udiv_rec E g ls1 ls2 qs rs : env * generator * cnf * word * word :=
   match ls1 with
@@ -672,27 +70,6 @@ Fixpoint mk_env_udiv_rec E g ls1 ls2 qs rs : env * generator * cnf * word * word
               (E_tl, g_tl, (catrev (catrev (catrev cs_tl cs_sub2) cs_and) cs_uge), lrs_tl, lqs_tl)
   end.       
 
-(*
-Fixpoint mk_env_udiv_rec (E: env) (g:generator) ls1 ls2 qs rs : env * generator * cnf * word * word :=
-  match ls1 with
-  | [::] => (E, g, [::], qs, rs)
-  | ls1_hd :: ls1_tl =>
-    let '(E_tl, g_tl, cs_tl, lrs_tl, lqs_tl) := mk_env_udiv_rec E g ls1_tl ls2 qs rs in
-    let di := dropmsl (joinlsl ls1_hd lrs_tl) in
-    let '(E_hd, g_hd, cs_hd, lrs_hd) := mk_env_uge E_tl g_tl di ls2 in
-    let qi := dropmsl (joinlsl lrs_hd lqs_tl) in
-    if (lrs_hd == lit_tt) then
-      let '(E_sub, g_sub, cs_sub, lrs_sub) := mk_env_sub E_hd g_hd di ls2 in
-      (E_sub, g_sub, (catrev (catrev cs_tl cs_hd) cs_sub), qi, lrs_sub)
-    else if (lrs_hd == lit_ff) then
-           (E_hd, g_hd, catrev cs_tl cs_hd, qi, di)
-         else let '(E_and, g_and, cs_and, lrs_and) := mk_env_and E_hd g_hd (copy (size ls2) lrs_hd) ls2 in
-              let '(E_sub2, g_sub2, cs_sub2, lrs_sub2) := mk_env_sub E_and g_and di lrs_and in
-              (E_sub2, g_sub2, (catrev (catrev (catrev cs_tl cs_hd) cs_and) cs_sub2), qi, lrs_sub2)
-  end.
- *)
-
-
 Definition mk_env_udiv E g ls1' ls2 :=
   let ls1 := rev ls1' in
   let '(E_eq, g_eq, cs_eq, lrs_eq) := mk_env_eq E g ls2 (copy (size ls2) lit_ff) in
@@ -708,6 +85,9 @@ Definition mk_env_udiv E g ls1' ls2 :=
          let '(E_and, g_and, cs_and, lrs_and) := mk_env_and E_udivr g_udivr (copy (size lqs_udivr) (neg_lit lrs_eq)) lqs_udivr  in
          let '(E_ite, g_ite, cs_ite, lrs_ite) := mk_env_ite E_and g_and lrs_eq (rev lrs_udivr) lrs_udivr in
          (E_ite, g_ite, catrev (catrev (catrev cs_ite cs_and) cs_udivr) cs_eq, lrs_and, lrs_ite).
+
+Definition mk_env_udiv' E g ls1 ls2 :=
+  let '(E_udiv, g_udiv, cs_udiv, q_udiv, r_udiv) := mk_env_udiv E g ls1 ls2 in (E_udiv, g_udiv, cs_udiv, q_udiv).
 
 Lemma bit_blast_sub_size_ss : forall g ls1 ls2 g' cs' lrs,
     bit_blast_sub g ls1 ls2  = (g', cs', lrs) -> size ls1 = size ls2 -> size lrs = size ls2.
@@ -1000,6 +380,19 @@ Proof.
         by rewrite -Hszlsbs2 Hbs20.
 Qed.
 
+Lemma bit_blast_udiv_correct' g ls1 ls2 g' cs qlrs E bs1 bs2 :
+  bit_blast_udiv' g ls1 ls2 = (g', cs, qlrs) ->
+  size ls1 = size ls2 ->
+  enc_bits E ls1 bs1 ->
+  enc_bits E ls2 bs2 ->
+  interp_cnf E (add_prelude cs) ->
+  enc_bits E qlrs (udivB bs1 bs2).1.
+Proof.
+  rewrite /bit_blast_udiv'. case Hbb : (bit_blast_udiv g ls1 ls2) => [[[g_u cs_u] q_u] r_u].
+  case => _ <- <-. move => Hs He1 He2 Hi. move : (bit_blast_udiv_correct Hbb Hs He1 He2 Hi) => [Hl Hr]. 
+  done.
+Qed.
+  
 Lemma mk_env_udiv_rec_is_bit_blast_udiv_rec: forall ls1 E g ls2 lq lr g' cs qlrs rlrs E',
   mk_env_udiv_rec E g ls1 ls2 lq lr = (E', g', cs, qlrs, rlrs) ->
   bit_blast_udiv_rec g ls1 ls2 lq lr = (g', cs, qlrs, rlrs).
@@ -1032,6 +425,15 @@ Proof.
   case (lrs_eq == lit_ff); by case => _ <- <- <- <- .
 Qed.  
 
+Lemma mk_env_udiv_is_bit_blast_udiv' : forall ls1 E g ls2 g' cs qlrs E',
+  mk_env_udiv' E g ls1 ls2 = (E', g', cs, qlrs) ->
+  bit_blast_udiv' g ls1 ls2  = (g', cs, qlrs).
+Proof.
+  move => ls1 E g ls2 g' cs qlrs E'. rewrite /mk_env_udiv' /bit_blast_udiv'. 
+  case Hmk : (mk_env_udiv E g ls1 ls2) => [[[[Emk gmk] csmk] qmk] rmk].
+  case => _ <- <- <-. by rewrite (mk_env_udiv_is_bit_blast_udiv Hmk).
+Qed.
+  
 Lemma mk_env_udiv_rec_newer_gen :
   forall ls1 E g ls2 lq lr E' g' cs lqs lrs,
     mk_env_udiv_rec E g ls1 ls2 lq lr = (E', g', cs, lqs, lrs) ->
@@ -1076,6 +478,16 @@ Proof.
   exact : (pos_leb_trans Hneweq Hnewudivr).
   move : (mk_env_ite_newer_gen Hmkite) => Hnewite. move : (mk_env_and_newer_gen Hmkand) => Hnewand. move: (mk_env_udiv_rec_newer_gen Hmkudivr) => Hnewudivr. move : (mk_env_eq_newer_gen Hmkeq) => Hneweq. 
   exact : (pos_leb_trans (pos_leb_trans Hneweq Hnewudivr) (pos_leb_trans Hnewand Hnewite)).
+Qed.
+
+Lemma mk_env_udiv_newer_gen' :
+  forall ls1 E g ls2 E' g' cs lqs,
+    mk_env_udiv' E g ls1 ls2 = (E', g', cs, lqs) ->
+    (g <=? g')%positive.
+Proof.
+  move => ls1 E g ls2 E' g' cs lqs. rewrite /mk_env_udiv'.
+  dcase (mk_env_udiv E g ls1 ls2) => [[[[[E_u] g_u] cs_u] lqs_u] lrs_u] Hmku.
+  case => _ <- _ _. rewrite (mk_env_udiv_newer_gen Hmku)//.
 Qed.
 
 Lemma mk_env_udiv_rec_newer_res :
@@ -1159,11 +571,23 @@ Proof.
   have Hnewcp : (newer_than_lits g_udivr (copy (size lqs_udivr) (neg_lit lrs_eq))) by rewrite newer_than_lits_copy; last by rewrite newer_than_lit_neg (newer_than_lit_le_newer (mk_env_eq_newer_res Hmkeq) Hnewudivr).
   have Hnewrev : (newer_than_lits g_eq (rev ls1)) by rewrite (newer_than_lits_rev (newer_than_lits_le_newer Hls1 Hneweq)).
   have Hnewcpeq : (newer_than_lits g_eq (copy (size (rev ls1)) lit_ff)) by rewrite newer_than_lits_copy; last by rewrite -newer_than_lit_tt_ff (newer_than_lit_le_newer Htt Hneweq).
-  
   move/andP : (mk_env_udiv_rec_newer_res Hmkudivr (newer_than_lit_le_newer Htt Hneweq) Hnewrev (newer_than_lits_le_newer Hls2 Hneweq) Hnewcpeq Hnewcpeq) => [Hnewq Hnewr].
   by rewrite (newer_than_lits_le_newer (mk_env_and_newer_res Hmkand (newer_than_lit_le_newer Htt Hgudivr) Hnewcp Hnewr) Hnewite).
 Qed.
 
+Lemma mk_env_udiv_newer_res' :
+  forall ls1 E g ls2 E' g' cs lqs,
+    mk_env_udiv' E g ls1 ls2  = (E', g', cs, lqs) ->
+    newer_than_lit g lit_tt ->
+    newer_than_lits g ls1 ->
+    newer_than_lits g ls2 ->
+    newer_than_lits g' lqs.
+Proof.
+  move => ls1 E g ls2 E' g' cs lqs Hmk Hnlt Hnl1 Hnl2. move : Hmk; rewrite /mk_env_udiv'.
+  dcase (mk_env_udiv E g ls1 ls2) => [[[[[E_u] g_u] cs_u] lqs_u] lrs_u] Hmku.
+  case => _ <- _ <-. by move :(mk_env_udiv_newer_res Hmku Hnlt Hnl1 Hnl2) => /andP [Hl Hr]. 
+Qed.
+  
 Lemma mk_env_udiv_rec_newer_cnf :
   forall ls1 E g ls2 lq lr E' g' cs lqs lrs,
     mk_env_udiv_rec E g ls1 ls2 lq lr = (E', g', cs, lqs, lrs) ->
@@ -1355,6 +779,20 @@ Proof.
     by rewrite (newer_than_cnf_le_newer Hncnfand Hnewite).
 Qed.
 
+
+Lemma mk_env_udiv_newer_cnf' :
+  forall ls1 E g ls2 E' g' cs lqs,
+    mk_env_udiv' E g ls1 ls2 = (E', g', cs, lqs) ->
+    newer_than_lit g lit_tt ->
+    newer_than_lits g ls1 ->
+    newer_than_lits g ls2 ->
+    newer_than_cnf g' cs.
+Proof.
+  move => ls1 E g ls2 E' g' cs lqs.
+  rewrite /mk_env_udiv'. case Hmk : (mk_env_udiv E g ls1 ls2) => [[[[E_u g_u] cs_u] lqs_u] lrs_u].
+  case => _ <- <- _. apply : (mk_env_udiv_newer_cnf Hmk).
+Qed.
+  
 (* This is a deprecated version of the above lemma that requires no size assumptions. *)
 (*
 Lemma mk_env_udiv_newer_cnf :
@@ -1416,11 +854,6 @@ Proof.
   elim => [|ls1hd ls1tl IH] E g ls2 lq lr E' g' cs lqs lrs.
   - by case => <- _ _ _. 
   - rewrite/=.
-    (*dcase (mk_env_udiv_rec E g ls1tl ls2 lq lr) => [[[[[E_tl g_tl] cs_tl] lrs_tl] lqs_tl] Hmkudiv].
-    dcase (mk_env_uge E_tl g_tl (dropmsl (joinlsl ls1hd lrs_tl)) ls2) => [[[[E_hd g_hd] cs_hd] lrs_hd] Hmkuge].
-    dcase (mk_env_sub E_hd g_hd (dropmsl (joinlsl ls1hd lrs_tl)) ls2) => [[[[E_sub g_sub] cs_sub] lrs_sub] Hmksub].
-    dcase (mk_env_and E_hd g_hd (copy (size ls2) lrs_hd) ls2) => [[[[E_and g_and] cs_and] lrs_and] Hmkand].
-    dcase (mk_env_sub E_and g_and (dropmsl (joinlsl ls1hd lrs_tl)) lrs_and) => [[[[E_sub2 g_sub2] cs_sub2] lrs_sub2] Hmksub2].*)
     dcase (mk_env_uge E g (dropmsl (joinlsl ls1hd lr)) ls2) => [[[[E_hd g_hd] cs_hd] lrs_hd] Hmkuge].
     dcase (mk_env_sub E_hd g_hd (dropmsl (joinlsl ls1hd lr)) ls2) => [[[[E_sub g_sub] cs_sub] lrs_sub] Hmksub].
     dcase (mk_env_udiv_rec E_sub g_sub ls1tl ls2 (dropmsl (joinlsl lrs_hd lq)) lrs_sub) =>[[[[[E_tl g_tl] cs_tl] lrs_tl] lqs_tl] Hmkudiv].
@@ -1431,7 +864,6 @@ Proof.
     dcase (mk_env_udiv_rec E_sub2 g_sub2 ls1tl ls2 (dropmsl (joinlsl lrs_hd lq)) lrs_sub2) =>
     [[[[[E_tl3 g_tl3] cs_tl3] lrs_tl3] lqs_tl3] Hmkudiv3].
     move => Hres .  
-    
     move : (mk_env_uge_preserve Hmkuge) => HE0E1g0.
     move : (mk_env_sub_preserve Hmksub) => HE1E2g1.
     move : (IH _ _ _ _ _ _ _ _ _ _ Hmkudiv ) => HE2E3g.
@@ -1489,6 +921,16 @@ Proof.
     exact : (env_preserve_trans HEEand (env_preserve_le HEandEitegand Hggand)).
 Qed.
 
+Lemma mk_env_udiv_preserve' :
+  forall E g ls1 ls2 E' g' cs lqs,
+    mk_env_udiv' E g ls1 ls2 = (E', g', cs, lqs) ->
+    env_preserve E E' g.
+Proof.
+  move => E g ls1 ls2 E' g' cs lqs. rewrite /mk_env_udiv'.
+  case Hmk : (mk_env_udiv E g ls1 ls2) => [[[[E_u g_u] cs_u] lqs_u] lrs_u].
+  case => <- _ _ _. apply : (mk_env_udiv_preserve Hmk).
+Qed.
+  
 Lemma mk_env_udiv_rec_sat :
   forall ls1 E g ls2 lq lr E' g' cs lqs lrs,
     mk_env_udiv_rec E g ls1 ls2 lq lr = (E', g', cs, lqs, lrs) ->
@@ -1561,7 +1003,6 @@ Proof.
     rewrite HEhdcshd in HEtl2cshdeq.
     move : (mk_env_and_newer_res Hmkand (newer_than_lit_le_newer Htt Hg0g1) (newer_than_lits_copy _ Hlrshd) (newer_than_lits_le_newer Hls2 Hg0g1)) => Hgandlrsand.
     move : (mk_env_sub_sat Hmksub2 (newer_than_lit_le_newer Hff (pos_leb_trans Hg0g1 Hg1g2'')) (newer_than_lits_le_newer Hdjlr0 (pos_leb_trans Hg0g1 Hg1g2'')) Hgandlrsand) => HEsub2cssub2.
-    
     move :Hres;
       case : (lrs_hd == lit_tt); case :(lrs_hd == lit_ff); move => [] <- _ <- _ _; rewrite !interp_cnf_catrev; try by rewrite HE2E3g Hcssubeq Hcshdeq.
     by rewrite HE2E3'g HEtl2cshdeq.
@@ -1748,6 +1189,19 @@ Proof.
     by rewrite (mk_env_ite_sat Hmkite (newer_than_lit_le_newer Htt Hggand) (newer_than_lit_le_newer Hgeqlrseq (pos_leb_trans Hnewudivr Hnewand)) Hnewerv (newer_than_lits_le_newer Hnewq Hnewand)).
 Qed.
 
+Lemma mk_env_udiv_sat' :
+  forall E g ls1 ls2 E' g' cs lqs,
+    mk_env_udiv' E g ls1 ls2 = (E', g', cs, lqs) ->
+    newer_than_lit g lit_tt ->
+    newer_than_lits g ls1 ->
+    newer_than_lits g ls2 ->
+    interp_cnf E' cs.
+Proof.
+  move => E g ls1 ls2 E' g' cs lqs. rewrite /mk_env_udiv'.
+  case Hmk : (mk_env_udiv E g ls1 ls2) => [[[[E_u g_u] cs_u] lqs_u] lrs_u].
+  case => <- _ <- _. apply : (mk_env_udiv_sat Hmk).
+Qed.
+  
 (* This is a deprecated version of the above lemma that requires no size assumptions. *)
 (*
 Lemma mk_env_udiv_sat :
